projection/payload_closureScript.sml
@@ -1,7 +1,6 @@
 (* Prepare for compilation to CakeML by switching from substitution semantics to environment semantics
    for function definitions *)
 open preamble choreoUtilsTheory payloadLangTheory;
-open endpoint_to_choiceTheory; (* For K0 *)
 
 val _ = new_theory "payload_closure";
 
@@ -13,23 +12,9 @@ Definition written_var_names_endpoint_def:
 ∧ (written_var_names_endpoint (Let v f vl e) = v::written_var_names_endpoint e)
 ∧ (written_var_names_endpoint (Fix dv e) = written_var_names_endpoint e)
 ∧ (written_var_names_endpoint (Call dv) = [])
-∧ (written_var_names_endpoint (Letrec dv vars e1) = written_var_names_endpoint e1)
+∧ (written_var_names_endpoint (Letrec dv vars e1) =
+   written_var_names_endpoint e1 ++ MAP FST (FILTER ($¬ o SND) vars))
 ∧ (written_var_names_endpoint (FCall dv vars) = vars)
-End
-
-Definition written_var_names_endpoint_until_def:
-   (written_var_names_endpoint_until Nil = [])
-∧ (written_var_names_endpoint_until (Send p v n e) = written_var_names_endpoint_until e)
-∧ (written_var_names_endpoint_until (Receive p v d e) = v::written_var_names_endpoint_until e)
-∧ (written_var_names_endpoint_until (IfThen v e1 e2) = written_var_names_endpoint_until e1 ++ written_var_names_endpoint_until e2)
-∧ (written_var_names_endpoint_until (Let v f vl e) = v::written_var_names_endpoint_until e)
-∧ (written_var_names_endpoint_until (Fix dv e) =
-    if free_fix_names_endpoint(Fix dv e) = []
-    then []
-    else written_var_names_endpoint_until e)
-∧ (written_var_names_endpoint_until (Call dv) = [])
-∧ (written_var_names_endpoint_until (Letrec dv vars e1) = written_var_names_endpoint_until e1)
-∧ (written_var_names_endpoint_until (FCall dv vars) = vars)
 End
 
 Definition written_var_names_endpoint_before_def:
@@ -54,7 +39,7 @@ Definition written_var_names_endpoint_before_def:
    if dn = dv then
      []
    else
-     written_var_names_endpoint_before dn e1)
+     written_var_names_endpoint_before dn e1 ++ MAP FST (FILTER ($¬ o SND) vars))
 ∧ (written_var_names_endpoint_before dn (FCall dv vars) =
     if dn = dv then
        vars
@@ -64,22 +49,22 @@ Definition written_var_names_endpoint_before_def:
 End
 
 Definition compile_endpoint_def:
-    (compile_endpoint ar payloadLang$Nil = payloadLang$Nil) ∧
-    (compile_endpoint ar (Send p v n e) = Send p v n (compile_endpoint ar e)) ∧
-    (compile_endpoint ar (Receive p v l e) = Receive p v l (compile_endpoint ar e)) ∧
-    (compile_endpoint ar (IfThen v e1 e2) =
-     IfThen v (compile_endpoint ar e1) (compile_endpoint ar e2)) ∧
-    (compile_endpoint ar (Let v f vl e) =
-     Let v f vl (compile_endpoint ar e)) ∧
-    (compile_endpoint ar (Letrec dn vars e1) = Nil (* Source term should use fixpoint style *)) ∧
-    (compile_endpoint ar (FCall dn vars) = Nil (* Source term should use fixpoint style *)) ∧
-    (compile_endpoint ar (Fix dn e) =
+    (compile_endpoint uw ar payloadLang$Nil = payloadLang$Nil) ∧
+    (compile_endpoint uw ar (Send p v n e) = Send p v n (compile_endpoint uw ar e)) ∧
+    (compile_endpoint uw ar (Receive p v l e) = Receive p v l (compile_endpoint (FILTER ($≠ v) uw) ar e)) ∧
+    (compile_endpoint uw ar (IfThen v e1 e2) =
+     IfThen v (compile_endpoint uw ar e1) (compile_endpoint uw ar e2)) ∧
+    (compile_endpoint uw ar (Let v f vl e) =
+     Let v f vl (compile_endpoint (FILTER ($≠ v) uw) ar e)) ∧
+    (compile_endpoint uw ar (Letrec dn vars e1) = Nil (* Source term should use fixpoint style *)) ∧
+    (compile_endpoint uw ar (FCall dn vars) = Nil (* Source term should use fixpoint style *)) ∧
+    (compile_endpoint uw ar (Fix dn e) =
      let vars = nub'(written_var_names_endpoint e);
-         e' = compile_endpoint ((dn,vars)::ar) e
+         e' = compile_endpoint (FILTER (λv. ¬MEM v vars) uw) ((dn,vars)::ar) e
      in
-       Letrec dn vars e'
+       Letrec dn (MAP (λv. (v, ¬MEM v uw)) vars) e'
     ) ∧
-    (compile_endpoint ar (Call dn) =
+    (compile_endpoint uw ar (Call dn) =
      case ALOOKUP ar dn of
        SOME vars =>
          FCall dn vars
@@ -90,16 +75,16 @@ End
 Definition compile_network_def:
   compile_network NNil = NNil
 ∧ compile_network (NPar n1 n2) = NPar (compile_network n1) (compile_network n2)
-∧ compile_network (NEndpoint p s e) =
+∧ compile_network (payloadLang$NEndpoint p s e) =
   let
     (* In order to avoid having to deal with closures under potentially undefined variables,
        make sure all variables that will be written to are initialised. *)
     undefined_writes = FILTER (λx. x ∉ (FDOM s.bindings)) (nub'(written_var_names_endpoint e))
   in
-    NEndpoint p s
-      (FOLDL (λe v. Let v K0 [] e) (compile_endpoint [] e) undefined_writes)
+    NEndpoint p s (compile_endpoint undefined_writes [] e)
 End
 
+(*
 Definition compile_network_alt_def:
   compile_network_alt NNil = NNil
 ∧ compile_network_alt (NPar n1 n2) = NPar (compile_network_alt n1) (compile_network_alt n2)
@@ -112,5 +97,6 @@ Definition compile_network_alt_def:
     NEndpoint p (s with bindings := s.bindings |++ MAP (λx. (x,[0w])) undefined_writes)
                 (compile_endpoint [] e)
 End
+*)
 
 val _ = export_theory ();
